stripped old-fashioned terminators;

thys/GraphMarkingIBP/StackMark.thy
@@ -20,107 +20,107 @@ subsection {* Transitions *}
 
 definition (in graph)
   "Q1' s \<equiv> let (stk::('node list), mrk::('node set)) = s in {(stk'::('node list), mrk') . 
-           root = nil \<and> stk' = [] \<and> mrk' = mrk}";
+           root = nil \<and> stk' = [] \<and> mrk' = mrk}"
 
 definition (in graph)
-  "Q2' s \<equiv> let (stk::('node list), mrk::('node set)) = s in {(stk', mrk') . root \<noteq> nil \<and> stk' = [root] \<and> mrk' = mrk \<union> {root}}";
+  "Q2' s \<equiv> let (stk::('node list), mrk::('node set)) = s in {(stk', mrk') . root \<noteq> nil \<and> stk' = [root] \<and> mrk' = mrk \<union> {root}}"
 
 definition (in graph)
   "Q3' s \<equiv> let (stk, mrk) = s in {(stk', mrk') .  stk \<noteq> [] \<and> (\<exists> y . (hd stk, y) \<in> next \<and> 
-    y \<notin> mrk \<and> stk' = y # stk \<and> mrk' = mrk \<union> {y})}";
+    y \<notin> mrk \<and> stk' = y # stk \<and> mrk' = mrk \<union> {y})}"
 
 definition (in graph)
   "Q4' s \<equiv> let (stk, mrk) = s in {(stk', mrk') . stk \<noteq> [] \<and> 
-  (\<forall> y . (hd stk, y) \<in> next \<longrightarrow> y \<in> mrk) \<and> stk' = tl stk \<and> mrk' = mrk}";
+  (\<forall> y . (hd stk, y) \<in> next \<longrightarrow> y \<in> mrk) \<and> stk' = tl stk \<and> mrk' = mrk}"
 
 definition
-  "Q5' s \<equiv> let (stk, mrk) = s in {(stk', mrk') . stk = [] \<and> mrk' = mrk}";
+  "Q5' s \<equiv> let (stk, mrk) = s in {(stk', mrk') . stk = [] \<and> mrk' = mrk}"
 
 subsection {* Invariants *}
 
 definition
-  "Init' \<equiv> UNIV";
+  "Init' \<equiv> UNIV"
 
 definition
-  "Loop' \<equiv> { (stk, mrk) . distinct stk}";
+  "Loop' \<equiv> { (stk, mrk) . distinct stk}"
 
 definition
-  "Final' \<equiv> UNIV";
+  "Final' \<equiv> UNIV"
 
 definition [simp]:
   "StackMarkInv i = (case i of
       I.init  \<Rightarrow> Init' |
       I.loop  \<Rightarrow> Loop' |
-      I.final \<Rightarrow> Final')";
+      I.final \<Rightarrow> Final')"
 
 subsection {* Data refinement relations *}
 
 definition
-  "R1 \<equiv> \<lambda> (stk, mrk) . {(X, mrk') . mrk' = mrk}";
+  "R1 \<equiv> \<lambda> (stk, mrk) . {(X, mrk') . mrk' = mrk}"
 
 definition
-  "R2 \<equiv> \<lambda> (stk, mrk) . {(X, mrk') . X = {x . x \<in> set stk} \<and> (stk, mrk) \<in> Loop' \<and> mrk' = mrk}";
+  "R2 \<equiv> \<lambda> (stk, mrk) . {(X, mrk') . X = {x . x \<in> set stk} \<and> (stk, mrk) \<in> Loop' \<and> mrk' = mrk}"
 
 definition [simp]:
   "R i = (case i of
       I.init  \<Rightarrow> R1 |
       I.loop  \<Rightarrow> R2 |
-      I.final \<Rightarrow> R1)";
+      I.final \<Rightarrow> R1)"
 
 definition (in graph)
   "StackMark_rel = (\<lambda> (i, j) . (case (i, j) of
       (I.init, I.loop)  \<Rightarrow> Q1' \<squnion> Q2' |
       (I.loop, I.loop)  \<Rightarrow> Q3' \<squnion> Q4' |
       (I.loop, I.final) \<Rightarrow> Q5' |
-       _ \<Rightarrow> \<bottom>))";
+       _ \<Rightarrow> \<bottom>))"
 
 subsection {* Data refinement of the transitions *}
 
 theorem (in graph) init_nil [simp]:
-  "DataRefinement Init Q1 R1 R2 (demonic Q1')";
+  "DataRefinement Init Q1 R1 R2 (demonic Q1')"
    by (simp add: DataRefinement_def hoare_demonic Q1'_def Init_def 
-     R1_def Loop'_def R1_def R2_def Q1_def angelic_def subset_eq);
+     R1_def Loop'_def R1_def R2_def Q1_def angelic_def subset_eq)
    
 theorem (in graph) init_root [simp]:
-  "DataRefinement Init Q2 R1 R2 (demonic Q2')";
+  "DataRefinement Init Q2 R1 R2 (demonic Q2')"
 by (auto simp: DataRefinement_def hoare_demonic Q2'_def Init_def
      Loop'_def R1_def R2_def Q2_def angelic_def subset_eq)
 
 theorem (in graph) step1 [simp]:
-  "DataRefinement Loop Q3 R2 R2 (demonic Q3')";
+  "DataRefinement Loop Q3 R2 R2 (demonic Q3')"
   apply (simp add: DataRefinement_def hoare_demonic Loop_def 
-    Loop'_def R2_def Q3_def Q3'_def angelic_def subset_eq);
-  apply (simp add: simp_eq_emptyset);
+    Loop'_def R2_def Q3_def Q3'_def angelic_def subset_eq)
+  apply (simp add: simp_eq_emptyset)
 by (metis Collect_def List.set.simps(2) hd_in_set mem_def member_set distinct.simps(2))
 
 theorem (in graph) step2 [simp]:
-  "DataRefinement Loop Q4 R2 R2 (demonic Q4')";
+  "DataRefinement Loop Q4 R2 R2 (demonic Q4')"
   apply (simp add: DataRefinement_def hoare_demonic Loop_def 
-    Loop'_def R2_def Q4_def Q4'_def angelic_def subset_eq);
-  apply (simp add: simp_eq_emptyset);
-  apply clarify;
-  apply (case_tac a);
-  by auto;
+    Loop'_def R2_def Q4_def Q4'_def angelic_def subset_eq)
+  apply (simp add: simp_eq_emptyset)
+  apply clarify
+  apply (case_tac a)
+  by auto
 
 
 theorem (in graph) final [simp]:
-  "DataRefinement Loop Q5 R2 R1 (demonic Q5')";
+  "DataRefinement Loop Q5 R2 R1 (demonic Q5')"
   apply (simp add: DataRefinement_def hoare_demonic Loop_def 
-    Loop'_def R2_def R1_def Q5_def Q5'_def angelic_def subset_eq);
-  by (simp add: simp_eq_emptyset);
+    Loop'_def R2_def R1_def Q5_def Q5'_def angelic_def subset_eq)
+  by (simp add: simp_eq_emptyset)
 
 subsection {* Diagram data refinement *}
 
 theorem (in graph) StackMark_DataRefinement [simp]:
- "DgrDataRefinement SetMarkInv SetMark_rel R (dgr_demonic StackMark_rel)";
-  by (simp add: DgrDataRefinement_def dgr_demonic_def StackMark_rel_def SetMark_rel_def demonic_sup_inf SetMarkInv_def data_refinement_choice2);
+ "DgrDataRefinement SetMarkInv SetMark_rel R (dgr_demonic StackMark_rel)"
+  by (simp add: DgrDataRefinement_def dgr_demonic_def StackMark_rel_def SetMark_rel_def demonic_sup_inf SetMarkInv_def data_refinement_choice2)
 
 subsection {* Diagram correctness *}
 
 theorem (in graph) StackMark_correct:
-  "Hoare_dgr (dangelic R SetMarkInv) (dgr_demonic StackMark_rel) ((dangelic R SetMarkInv) \<sqinter> (- grd (step ((dgr_demonic StackMark_rel)))))";
-  apply (rule_tac T="SetMark_rel" in Diagram_DataRefinement);
-  apply auto;
-  by (rule SetMark_correct1);
+  "Hoare_dgr (dangelic R SetMarkInv) (dgr_demonic StackMark_rel) ((dangelic R SetMarkInv) \<sqinter> (- grd (step ((dgr_demonic StackMark_rel)))))"
+  apply (rule_tac T="SetMark_rel" in Diagram_DataRefinement)
+  apply auto
+  by (rule SetMark_correct1)
 
-end;
+end
