thys/GraphMarkingIBP/LinkMark.thy
@@ -31,12 +31,12 @@ locale pointer = node +
   assumes "(nil::'node) = nil"
 begin
   definition "next =  {(a, b) . (\<exists> i . link0 i a = b) \<and> a \<noteq> nil \<and> b \<noteq> nil \<and> label0 a = none}"
-end;
+end
 
 sublocale  pointer \<subseteq> graph "nil" "root" "next"
-  apply unfold_locales;
-  apply (unfold next_def);
-  by auto;
+  apply unfold_locales
+  apply (unfold next_def)
+  by auto
 
 text{*
 The locale pointer fixes the initial values for the variables $ \mathit{link}$ and $ \mathit{label}$ and
@@ -56,7 +56,7 @@ begin
 primrec
   label_0:: "('node \<Rightarrow> 'index) \<Rightarrow> ('node list) \<Rightarrow> ('node \<Rightarrow> 'index)" where 
    "label_0 lbl []      = lbl" |
-   "label_0 lbl (x # l) = label_0 (lbl(x := none)) l";
+   "label_0 lbl (x # l) = label_0 (lbl(x := none)) l"
 
 lemma label_cong [cong]: "f = g \<Longrightarrow> xs = ys \<Longrightarrow> pointer.label_0 n f xs = pointer.label_0 n g ys"
 by simp
@@ -64,7 +64,7 @@ by simp
 primrec
   link_0:: "('index \<Rightarrow> 'node \<Rightarrow> 'node) \<Rightarrow> ('node \<Rightarrow> 'index) \<Rightarrow> 'node \<Rightarrow> ('node list) \<Rightarrow> ('index \<Rightarrow> 'node \<Rightarrow> 'node)" where
   "link_0 lnk lbl p []       = lnk" |
-  "link_0 lnk lbl p (x # l)  = link_0 (lnk((lbl x) := ((lnk (lbl x))(x := p)))) lbl x l";
+  "link_0 lnk lbl p (x # l)  = link_0 (lnk((lbl x) := ((lnk (lbl x))(x := p)))) lbl x l"
 
 text{*
 The function $ \mathit{stack}$ defined bellow is the main data refinement relation connecting
@@ -76,34 +76,34 @@ primrec
   stack:: "('index \<Rightarrow> 'node \<Rightarrow> 'node) \<Rightarrow> ('node \<Rightarrow> 'index) \<Rightarrow> 'node \<Rightarrow> ('node list) \<Rightarrow> bool" where
   "stack lnk lbl x []       = (x = nil)" |
   "stack lnk lbl x (y # l)  = 
-      (x \<noteq> nil \<and> x = y \<and> \<not> x \<in> set l \<and> stack lnk lbl (lnk (lbl x) x) l)";
+      (x \<noteq> nil \<and> x = y \<and> \<not> x \<in> set l \<and> stack lnk lbl (lnk (lbl x) x) l)"
 
 
 lemma label_out_range0 [simp]:
-  "\<not> x \<in> set S \<Longrightarrow> label_0 lbl S x = lbl x";
-  apply (rule_tac P="\<forall> label . \<not> x \<in> set S \<longrightarrow> label_0 label S x = label x" in mp);
-  by (simp, induct_tac S, auto);
+  "\<not> x \<in> set S \<Longrightarrow> label_0 lbl S x = lbl x"
+  apply (rule_tac P="\<forall> label . \<not> x \<in> set S \<longrightarrow> label_0 label S x = label x" in mp)
+  by (simp, induct_tac S, auto)
 
 lemma link_out_range0 [simp]:
-  "\<not> x \<in> set S \<Longrightarrow> link_0 link label p S i x = link i x";
-  apply (rule_tac P="\<forall> link p . \<not> x \<in> set S \<longrightarrow> link_0 link label p S i x = link i x" in mp);
-  by (simp, induct_tac S, auto);
+  "\<not> x \<in> set S \<Longrightarrow> link_0 link label p S i x = link i x"
+  apply (rule_tac P="\<forall> link p . \<not> x \<in> set S \<longrightarrow> link_0 link label p S i x = link i x" in mp)
+  by (simp, induct_tac S, auto)
 
 
-lemma link_out_range [simp]: "\<not> x \<in> set S \<Longrightarrow> link_0 link (label(x := y)) p S = link_0 link label p S";
-  apply (rule_tac P="\<forall> link p . \<not> x \<in> set S \<longrightarrow> link_0 link (label(x := y)) p S = link_0 link label p S" in mp);
-  by (simp, induct_tac S, auto);
+lemma link_out_range [simp]: "\<not> x \<in> set S \<Longrightarrow> link_0 link (label(x := y)) p S = link_0 link label p S"
+  apply (rule_tac P="\<forall> link p . \<not> x \<in> set S \<longrightarrow> link_0 link (label(x := y)) p S = link_0 link label p S" in mp)
+  by (simp, induct_tac S, auto)
 
-lemma empty_stack [simp]: "stack link label nil S = (S = [])";
-  by (case_tac S, simp_all);
+lemma empty_stack [simp]: "stack link label nil S = (S = [])"
+  by (case_tac S, simp_all)
 
-lemma stack_out_link_range [simp]: "\<not> p \<in> set S \<Longrightarrow> stack (link(i := (link i)(p := q))) label x S = stack link label x S";
-  apply (rule_tac P = "\<forall> link x . \<not> p \<in> set S \<longrightarrow> stack (link(i := (link i)(p := q))) label x S = stack link label x S" in mp);
-  by (simp, induct_tac S, auto);
+lemma stack_out_link_range [simp]: "\<not> p \<in> set S \<Longrightarrow> stack (link(i := (link i)(p := q))) label x S = stack link label x S"
+  apply (rule_tac P = "\<forall> link x . \<not> p \<in> set S \<longrightarrow> stack (link(i := (link i)(p := q))) label x S = stack link label x S" in mp)
+  by (simp, induct_tac S, auto)
 
-lemma stack_out_label_range [simp]: "\<not> p \<in> set S \<Longrightarrow> stack link (label(p := q)) x S = stack link label x S";
-  apply (rule_tac P = "\<forall> link x . \<not> p \<in> set S \<longrightarrow> stack link (label(p := q)) x S = stack link label x S" in mp);
-  by (simp, induct_tac S, auto);
+lemma stack_out_label_range [simp]: "\<not> p \<in> set S \<Longrightarrow> stack link (label(p := q)) x S = stack link label x S"
+  apply (rule_tac P = "\<forall> link x . \<not> p \<in> set S \<longrightarrow> stack link (label(p := q)) x S = stack link label x S" in mp)
+  by (simp, induct_tac S, auto)
 
 definition
   "g mrk lbl ptr x \<equiv> ptr x \<noteq> nil \<and> ptr x \<notin> mrk \<and> lbl x = none"
@@ -116,19 +116,19 @@ subsection {* Transitions *}
 
 definition
   "Q1'' s \<equiv> let (p, t, lnk, lbl, mrk) = s in { (p', t', lnk', lbl', mrk') .
-      root = nil \<and> p' = nil \<and> t' = nil \<and> lnk' = lnk \<and> lbl' = lbl \<and> mrk' = mrk}";
+      root = nil \<and> p' = nil \<and> t' = nil \<and> lnk' = lnk \<and> lbl' = lbl \<and> mrk' = mrk}"
 
 
 definition
   "Q2'' s \<equiv> let (p, t, lnk, lbl, mrk) = s in { (p', t', lnk', lbl', mrk') .
-      root \<noteq> nil \<and> p' = root \<and> t' = nil \<and> lnk' = lnk \<and> lbl' = lbl \<and> mrk' = mrk \<union> {root}}";
+      root \<noteq> nil \<and> p' = root \<and> t' = nil \<and> lnk' = lnk \<and> lbl' = lbl \<and> mrk' = mrk \<union> {root}}"
 
 definition
   "Q3'' s \<equiv> let (p, t, lnk, lbl, mrk) = s in { (p', t', lnk', lbl', mrk') .
          p \<noteq> nil \<and> 
          (\<exists> i . g mrk lbl (lnk i) p \<and> 
             p' = lnk i p \<and> t' =  p \<and> lnk' =  lnk(i := (lnk i)(p := t)) \<and> lbl' = lbl(p := i) \<and>
-            mrk' = mrk \<union> {lnk i p})}";
+            mrk' = mrk \<union> {lnk i p})}"
 
 definition
   "Q4'' s  \<equiv> let (p, t, lnk, lbl, mrk) = s in { (p', t', lnk', lbl', mrk') .
@@ -141,27 +141,27 @@ definition
   "Q5'' s \<equiv> let (p, t, lnk, lbl, mrk) = s in { (p', t', lnk', lbl', mrk') .
            p \<noteq> nil \<and> 
           (\<forall> i . \<not> g mrk lbl (lnk i) p) \<and> t = nil \<and>
-           p' = nil \<and> t' = t \<and> lnk' =  lnk \<and> lbl' = lbl \<and> mrk' = mrk}";
+           p' = nil \<and> t' = t \<and> lnk' =  lnk \<and> lbl' = lbl \<and> mrk' = mrk}"
 
 definition
   "Q6'' s \<equiv> let (p, t, lnk, lbl, mrk) = s in {(p', t', lnk', lbl', mrk') . p = nil \<and>  
-         p' = p \<and> t' = t \<and> lnk' = lnk \<and> lbl' =  lbl \<and> mrk' = mrk}";
+         p' = p \<and> t' = t \<and> lnk' = lnk \<and> lbl' =  lbl \<and> mrk' = mrk}"
 
 subsection {* Invariants *}
 
 definition
-  "Init'' \<equiv> { (p, t, lnk, lbl, mrk) . lnk = link0 \<and> lbl = label0}";
+  "Init'' \<equiv> { (p, t, lnk, lbl, mrk) . lnk = link0 \<and> lbl = label0}"
 
 definition
-  "Loop'' \<equiv> UNIV";
+  "Loop'' \<equiv> UNIV"
 
 definition
-  "Final'' \<equiv> Init''";
+  "Final'' \<equiv> Init''"
 
 subsection {* Data refinement relations *}
 
 definition 
-  "R1' \<equiv> (\<lambda> (p, t, lnk, lbl, mrk) . {(stk, mrk') . (p, t, lnk, lbl, mrk) \<in> Init'' \<and> mrk' = mrk})";
+  "R1' \<equiv> (\<lambda> (p, t, lnk, lbl, mrk) . {(stk, mrk') . (p, t, lnk, lbl, mrk) \<in> Init'' \<and> mrk' = mrk})"
 
 definition  
   "R2' \<equiv> (\<lambda> (p, t, lnk, lbl, mrk) . {(stk, mrk') .  
@@ -171,13 +171,13 @@ definition
        link0 = link_0 lnk lbl p (tail stk) \<and> 
        label0 = label_0 lbl (tail stk) \<and>
        \<not> nil \<in> set stk \<and> 
-       mrk' = mrk})";
+       mrk' = mrk})"
 
 definition [simp]:
   "R' i = (case i of
       I.init  \<Rightarrow> R1' |
       I.loop  \<Rightarrow> R2' |
-      I.final \<Rightarrow> R1')";
+      I.final \<Rightarrow> R1')"
 
 subsection{* Diagram *}
 
@@ -186,122 +186,122 @@ definition
       (I.init, I.loop)  \<Rightarrow> Q1'' \<squnion> Q2'' |
       (I.loop, I.loop)  \<Rightarrow> Q3'' \<squnion> (Q4'' \<squnion> Q5'') |
       (I.loop, I.final) \<Rightarrow> Q6'' |
-       _ \<Rightarrow> \<bottom>))";
+       _ \<Rightarrow> \<bottom>))"
 
 definition [simp]:
   "LinkMarkInv i = (case i of
       I.init  \<Rightarrow> Init'' |
       I.loop  \<Rightarrow> Loop'' |
-      I.final \<Rightarrow> Final'')";
+      I.final \<Rightarrow> Final'')"
 
 subsection {* Data refinement of the transitions *}
 
 theorem init1 [simp]:
-  "DataRefinement Init' Q1' R1' R2' (demonic Q1'')";
+  "DataRefinement Init' Q1' R1' R2' (demonic Q1'')"
   by (simp add: DataRefinement_def hoare_demonic Q1''_def Init'_def Init''_def 
-       Loop''_def R1'_def R2'_def Q1'_def tail_def head_def angelic_def subset_eq);
+       Loop''_def R1'_def R2'_def Q1'_def tail_def head_def angelic_def subset_eq)
 
 theorem init2 [simp]:
-  "DataRefinement Init' Q2' R1' R2' (demonic Q2'')";
+  "DataRefinement Init' Q2' R1' R2' (demonic Q2'')"
   by (simp add: DataRefinement_def hoare_demonic Q2''_def Init'_def Init''_def 
-       Loop''_def R1'_def R2'_def Q2'_def tail_def head_def angelic_def subset_eq);
+       Loop''_def R1'_def R2'_def Q2'_def tail_def head_def angelic_def subset_eq)
 
 theorem step1 [simp]:
-  "DataRefinement Loop' Q3' R2' R2' (demonic Q3'')";
+  "DataRefinement Loop' Q3' R2' R2' (demonic Q3'')"
   apply (simp add: DataRefinement_def hoare_demonic Q3''_def Init'_def Init''_def 
-       Loop'_def R1'_def Q3'_def tail_def head_def angelic_def subset_eq);
-  apply (simp add: simp_eq_emptyset);
-  apply auto;
-  apply (unfold next_def);
-  apply (unfold R2'_def);
-  apply (simp add: simp_eq_emptyset);
-  apply safe;
-  apply simp;
-  apply (rule_tac x = "ac i (hd a) # a" in exI);
-  apply safe;
-  apply simp_all;
-  apply (simp add: g_def  neq_Nil_conv);
-  apply clarify;
-  apply (simp add: g_def  neq_Nil_conv);
-  apply (case_tac a);
-  apply (simp_all add: g_def  neq_Nil_conv);
-  apply (case_tac a);
-  apply simp_all;
-  apply (case_tac a);
-  by auto;
+       Loop'_def R1'_def Q3'_def tail_def head_def angelic_def subset_eq)
+  apply (simp add: simp_eq_emptyset)
+  apply auto
+  apply (unfold next_def)
+  apply (unfold R2'_def)
+  apply (simp add: simp_eq_emptyset)
+  apply safe
+  apply simp
+  apply (rule_tac x = "ac i (hd a) # a" in exI)
+  apply safe
+  apply simp_all
+  apply (simp add: g_def  neq_Nil_conv)
+  apply clarify
+  apply (simp add: g_def  neq_Nil_conv)
+  apply (case_tac a)
+  apply (simp_all add: g_def  neq_Nil_conv)
+  apply (case_tac a)
+  apply simp_all
+  apply (case_tac a)
+  by auto
 
 lemma neqif [simp]: "x \<noteq> y \<Longrightarrow> (if y = x then a else b) = b"
-  apply (case_tac "y \<noteq> x");
-  apply simp_all;
-  done;
+  apply (case_tac "y \<noteq> x")
+  apply simp_all
+  done
 
 theorem step2 [simp]:
-  "DataRefinement Loop' Q4' R2' R2' (demonic Q4'')";
+  "DataRefinement Loop' Q4' R2' R2' (demonic Q4'')"
   apply (simp add: DataRefinement_def hoare_demonic Q4''_def Init'_def Init''_def 
-       Loop'_def Q4'_def angelic_def subset_eq);
-  apply (simp add: simp_eq_emptyset);
-  apply safe;
-  apply (unfold next_def);
-  apply (unfold R2'_def);
-  apply (simp_all add: neq_Nil_conv);
-  apply auto [1];
-  apply (case_tac ysa);
-  apply (simp add: head_def);
-  apply (simp add: head_def);
-  apply (case_tac a);
-  apply simp;
-  apply simp;
-  apply (unfold g_def);
-  by auto;
+       Loop'_def Q4'_def angelic_def subset_eq)
+  apply (simp add: simp_eq_emptyset)
+  apply safe
+  apply (unfold next_def)
+  apply (unfold R2'_def)
+  apply (simp_all add: neq_Nil_conv)
+  apply auto [1]
+  apply (case_tac ysa)
+  apply (simp add: head_def)
+  apply (simp add: head_def)
+  apply (case_tac a)
+  apply simp
+  apply simp
+  apply (unfold g_def)
+  by auto
 
-lemma setsimp: "a = c \<Longrightarrow> (x \<in> a) = (x \<in> c)"; 
-  apply simp;
-  done;
+lemma setsimp: "a = c \<Longrightarrow> (x \<in> a) = (x \<in> c)" 
+  apply simp
+  done
 
 theorem step3 [simp]:
-  "DataRefinement Loop' Q4' R2' R2' (demonic Q5'')";
+  "DataRefinement Loop' Q4' R2' R2' (demonic Q5'')"
   apply (simp add: DataRefinement_def hoare_demonic Q5''_def Init'_def Init''_def 
-       Loop'_def Q4'_def angelic_def subset_eq);
-  apply (unfold R2'_def);
-  apply (unfold next_def);
-  apply (simp add: simp_eq_emptyset);
-  apply (unfold g_def);
-  apply safe; 
-  apply (simp_all add: head_def tail_def);
-  by auto;
+       Loop'_def Q4'_def angelic_def subset_eq)
+  apply (unfold R2'_def)
+  apply (unfold next_def)
+  apply (simp add: simp_eq_emptyset)
+  apply (unfold g_def)
+  apply safe 
+  apply (simp_all add: head_def tail_def)
+  by auto
 
 theorem final [simp]:
-  "DataRefinement Loop' Q5' R2' R1' (demonic Q6'')";
+  "DataRefinement Loop' Q5' R2' R1' (demonic Q6'')"
    apply (simp add: DataRefinement_def hoare_demonic Q6''_def Init'_def Init''_def 
-       Loop'_def R2'_def R1'_def Q5'_def angelic_def subset_eq neq_Nil_conv tail_def head_def);
-  apply (simp add: simp_eq_emptyset);
-   apply safe;
-   by simp_all;
+       Loop'_def R2'_def R1'_def Q5'_def angelic_def subset_eq neq_Nil_conv tail_def head_def)
+  apply (simp add: simp_eq_emptyset)
+   apply safe
+   by simp_all
 
 subsection {* Diagram data refinement *}
 
 theorem LinkMark_DataRefinement [simp]:
- "DgrDataRefinement (dangelic R SetMarkInv) StackMark_rel R' (dgr_demonic LinkMark_rel)";
-  apply (rule_tac P = "StackMarkInv" in DgrDataRefinement_mono);
-  apply (simp add: le_fun_def dangelic_def SetMarkInv_def angelic_def R1_def R2_def Init'_def Final'_def mem_def le_bool_def);
-  apply auto;
-  apply (unfold simp_set_function);
-  apply auto;
-  apply (simp add: DgrDataRefinement_def dgr_demonic_def LinkMark_rel_def StackMark_rel_def demonic_sup_inf data_refinement_choice2);
-  apply (rule data_refinement_choice2);
-  apply auto;
-  apply (rule data_refinement_choice);
-  by auto;
+ "DgrDataRefinement (dangelic R SetMarkInv) StackMark_rel R' (dgr_demonic LinkMark_rel)"
+  apply (rule_tac P = "StackMarkInv" in DgrDataRefinement_mono)
+  apply (simp add: le_fun_def dangelic_def SetMarkInv_def angelic_def R1_def R2_def Init'_def Final'_def mem_def le_bool_def)
+  apply auto
+  apply (unfold simp_set_function)
+  apply auto
+  apply (simp add: DgrDataRefinement_def dgr_demonic_def LinkMark_rel_def StackMark_rel_def demonic_sup_inf data_refinement_choice2)
+  apply (rule data_refinement_choice2)
+  apply auto
+  apply (rule data_refinement_choice)
+  by auto
 
 subsection {* Diagram correctness *}
 
 theorem LinkMark_correct:
-  "Hoare_dgr (dangelic R' (dangelic R SetMarkInv)) (dgr_demonic LinkMark_rel) ((dangelic R' (dangelic R SetMarkInv)) \<sqinter> (- grd (step ((dgr_demonic LinkMark_rel)))))";
-  apply (rule_tac T="StackMark_rel" in Diagram_DataRefinement);
-  apply auto;
-  by (rule StackMark_correct);
+  "Hoare_dgr (dangelic R' (dangelic R SetMarkInv)) (dgr_demonic LinkMark_rel) ((dangelic R' (dangelic R SetMarkInv)) \<sqinter> (- grd (step ((dgr_demonic LinkMark_rel)))))"
+  apply (rule_tac T="StackMark_rel" in Diagram_DataRefinement)
+  apply auto
+  by (rule StackMark_correct)
 
 
-end;
+end
 
-end;
+end
